finished stepping through instructions

theories/examples/switcher/switcher.v
@@ -1,7 +1,7 @@
 From iris.algebra Require Import frac.
 From iris.proofmode Require Import proofmode.
 From cap_machine Require Import rules proofmode.
-From cap_machine Require Export clear_stack clear_registers.
+From cap_machine Require Export clear_stack clear_registers bitblast.
 
 Section Switcher.
   Context `{MP: MachineParameters}.
@@ -128,14 +128,6 @@ Section Switcher.
 
   Definition switcher_instrs : list Word :=
     switcher_call_instrs ++ switcher_return_instrs.
-
-  Definition encode_entry_point (nargs entry_point_offset : Z) : Z :=
-    let args := Z.land nargs 7 in
-    let off := Z.shiftl entry_point_offset 3 in
-    (Z.lor off args).
-
-  Definition decode_entry_point (entry_point : Z) : (Z * Z) :=
-    ( Z.land entry_point 7, Z.shiftr entry_point 3).
 
 
   Class switcherLayout : Type :=
