theories/bitblast.v
@@ -541,12 +541,17 @@ Tactic Notation "bitblast" ident(H) "with" constr(i) "as" ident(H') :=
 Tactic Notation "bitblast" ident(H) "with" constr(i) :=
   let H' := fresh "H" in bitblast H with i as H'.
 
-  Definition encode_entry_point (nargs entry_point_offset : Z) : Z :=
-    let args := Z.land nargs 7 in
-    let off := Z.shiftl entry_point_offset 3 in
-    (Z.lor off args).
+Definition encode_entry_point (nargs entry_point_offset : Z) : Z :=
+  let args := Z.land nargs 7 in
+  let off := Z.shiftl entry_point_offset 3 in
+  (Z.lor off args).
 
-Goal forall nargs off_entry, (0 ≤ nargs ≤ 7)%Z -> ( (Z.land (encode_entry_point nargs off_entry) 7)) = nargs.
+Definition decode_entry_point (entry_point : Z) : (Z * Z) :=
+  ( Z.land entry_point 7, Z.shiftr entry_point 3).
+
+Lemma encode_entry_point_eq_nargs nargs off_entry :
+  (0 ≤ nargs ≤ 7)%Z -> ( (Z.land (encode_entry_point nargs off_entry) 7)) = nargs.
+Proof.
   intros.
   rewrite /encode_entry_point.
   bitblast.
@@ -560,7 +565,10 @@ Goal forall nargs off_entry, (0 ≤ nargs ≤ 7)%Z -> ( (Z.land (encode_entry_po
   destruct (decide (nargs = 7)); simplify_eq; first bitblast.
   lia.
 Qed.
-Goal forall nargs off_entry, ( (encode_entry_point nargs off_entry ≫ 3)) = off_entry.
+
+Lemma encode_entry_point_eq_off nargs off_entry :
+  ( (encode_entry_point nargs off_entry ≫ 3)) = off_entry.
+Proof.
   intros.
   rewrite /encode_entry_point.
   bitblast.
